\chapter{Regulator DMC MIMO}

\section{Implementacja DMC}

\begin{equation}
	y(k) = 
	\begin{bmatrix}
		y_{1}(\textrm{k}) \\
		y_{2}(\textrm{k}) \\
	\end{bmatrix}
\end{equation}

\begin{equation}
	y^{\text{\textrm{zad}}}(k) = 
	\begin{bmatrix}
		y_{1}^{\textrm{zad}}(\textrm{k}) \\
		y_{2}^{\textrm{zad}}(\textrm{k}) \\
	\end{bmatrix}
\end{equation}

\begin{equation}
	u(k) = 
	\begin{bmatrix}
		u_{1}(\textrm{k}) \\
		u_{2}(\textrm{k}) \\
	\end{bmatrix}
\end{equation}

\begin{equation}
	S_l = 
	\begin{bmatrix}
		s_{l}^{\textrm{11}} & s_{l}^{\textrm{12}} \\
		s_{l}^{\textrm{21}} & s_{l}^{\textrm{22}} \\
	\end{bmatrix}
	,l = 1...D
\end{equation}

\begin{equation}
	M = 
	\begin{bmatrix}
		S_1 & 0 & \hdots & 0 \\
		S_2 & S_1 & \hdots & 0 \\
		\vdots & \vdots &\ddots & \vdots \\
		S_N & S_{N-1} & \hdots & S_{N-N_{\text{u}}+1} \\
	\end{bmatrix}
\end{equation}

\begin{equation}
	M^{\text{P}} = 
	\begin{bmatrix}
		S_2-S_1 & S_3-S_2 & \hdots & S_D-S_{D-1} \\
		S_3-S_1 & S_4-S_2 & \hdots & S_{D+1}-S_{D-1} \\
		\vdots & \vdots & \ddots & \vdots \\
		S_{N+1}-S_1 & S_{N+2}-S_2 & \hdots & S_{N+D-1}-S_{D-1} \\
	\end{bmatrix}
\end{equation}

\begin{equation}
	K = (M^{\textrm{T}}M+\lambda I)^{-1}M^{\textrm{T}} 
\end{equation}

\begin{equation}
	Y^\textrm{0}(k) = Y(k)+M^{\textrm{P}} \Delta U^{\textrm{P}}(k)
\end{equation}

\begin{equation}
	\Delta U(k) = K( Y^{\textrm{zad}}(k) - Y^\textrm{0}(k) )
\end{equation}

\section{Strojenie DMC}

\section{Regulacja DMC}